theories/SLFStruct.v
@@ -1,0 +1,914 @@
+(**
+
+Separation Logic Foundations
+
+Chapter: "Struct".
+
+Author: Arthur Charguéraud.
+License: CC-by 4.0.
+
+*)
+
+Set Implicit Arguments.
+From Sep Require Import SLFDirect SLFExtra.
+
+Implicit Types h : heap.
+Implicit Types P : Prop.
+Implicit Types H : hprop.
+Implicit Types Q : val->hprop.
+
+(*
+
+(* ####################################################### *)
+(* ####################################################### *)
+(* ####################################################### *)
+(** * Chapter in a rush *)
+
+(** This chapter introduces
+
+    - records
+    - arrays
+    - n-ary functions
+
+*)
+
+
+(* ####################################################### *)
+(** ** Semantics of the allocation of consecutive cells *)
+
+val_uninitialized
+
+=> restriction on read is possible
+
+Fixpoint nat_seq p k =
+  match k with
+
+Fixpoint hfold_list F L =
+  match L with
+
+Definition hcells n p =
+  hfold_list (fun q => q ~~> val_uninitialized) (seq p k).
+
+Implicit Types n : int
+
+
+(* ####################################################### *)
+(** ** Specification of the allocation of consecutive cells *)
+
+Lemma triple_alloc : forall n,
+  n >= 0 ->
+  triple (val_alloc n)
+    \[]
+    (fun r => \exists l, \[r = val_loc l /\ l <> null] \* Alloc (abs n) l).
+Proof using.
+  intros. applys triple_of_hoare. intros HF.
+  esplit; split. { applys~ hoare_alloc. } { xsimpl*. }
+Qed.
+
+Lemma triple_dealloc : forall n l,
+  n >= 0 ->
+  triple (val_dealloc n l)
+    (Dealloc (abs n) l)
+    (fun r => \[r = val_unit]).
+Proof using.
+  intros. applys triple_of_hoare. intros HF.
+  esplit; split. { applys~ hoare_dealloc. } { xsimpl*. }
+Qed.
+
+
+Fixpoint Alloc (k:nat) (l:loc) : hprop :=
+  match k with
+  | O => \[]
+  | S k' => l ~~~> val_uninitialized \* (Alloc k' (S l)%nat)
+  end.
+
+Lemma Alloc_zero_eq : forall l,
+  Alloc O l = \[].
+Proof using. auto. Qed.
+
+Lemma Alloc_succ_eq : forall l k,
+  Alloc (S k) l = l ~~~> val_uninitialized \* Alloc k (S l)%nat.
+Proof using. auto. Qed.
+
+Global Opaque Alloc.
+
+Hint Rewrite Alloc_zero_eq Alloc_succ_eq : rew_Alloc.
+
+Tactic Notation "rew_Alloc" :=
+  autorewrite with rew_Alloc.
+
+Lemma Alloc_split_eq : forall k1 (k:nat) p,
+  (k1 <= k)%nat ->
+  Alloc k p = Alloc k1 p \* Alloc (k-k1)%nat (p + k1)%nat.
+Proof using.
+  Transparent loc field. unfold field.
+  intros k1 k. gen k1. induction k; introv N.
+  {math_rewrite (k1 = 0%nat). rew_Alloc. rew_heap~. }
+  { destruct k1 as [|k1']; rew_nat.
+    { rew_Alloc. rew_heap~. }
+    { rew_Alloc. rewrite (IHk k1'); [|math]. rew_heap~. } }
+Qed.
+
+Arguments Alloc_split_eq : clear implicits.
+
+Lemma Alloc_split_inv : forall k1 k2 p,
+  Alloc k1 p \* Alloc k2 (p + k1)%nat ==> Alloc (k1+k2)%nat p.
+Proof using.
+  intros. rewrites (Alloc_split_eq k1 (k1+k2)%nat p); [|math]. rew_nat~.
+Qed.
+
+
+
+
+(* ########################################################### *)
+(** ** Definition of record fields *)
+
+Definition field : Type := nat.
+
+Definition hfield (l:loc) (k:field) (v:val) : hprop :=
+  (l+k)%nat ~~> v \* \[ l <> null ].
+
+Notation "l `. k '~~>' v" := (hfield l k v)
+  (at level 32, k at level 0, no associativity,
+   format "l `. k  '~~>'  v") : heap_scope.
+
+Lemma hfield_not_null : forall l k v,
+  (l`.k ~~> v) ==> (l`.k ~~> v) \* \[l <> null].
+Proof using.
+  intros. subst. unfold hfield. xchanges~ hsingle_not_null.
+Qed.
+
+
+
+
+(* ########################################################### *)
+(** ** Specification of record operations *)
+
+
+Parameter triple_get_field : forall l f v,
+  triple ((val_get_field f) l)
+    (l`.f ~~> v)
+    (fun r => \[r = v] \* (l`.f ~~> v)).
+
+Parameter triple_set_field : forall v1 l f v2,
+  triple ((val_set_field f) l v2)
+    (l`.f ~~> v1)
+    (fun _ => l`.f ~~> v2).
+
+Hint Resolve triple_get_field triple_set_field : triple.
+
+
+
+
+(* ####################################################### *)
+(** ** Representation predicate for a record *)
+
+
+Definition head : field := 0%nat.
+Definition tail : field := 1%nat.
+
+
+Definition MCell (x:val) (q:loc) (p:loc) : hprop :=
+  (p`.head ~~> x) \* (p`.tail ~~> q).
+
+
+
+(* ####################################################### *)
+(** ** Representation predicate for an array *)
+
+
+(* ---------------------------------------------------------------------- *)
+(** Representation *)
+
+Fixpoint Array (L:list val) (p:loc) : hprop :=
+  match L with
+  | nil => \[]
+  | x::L' => (p ~~~> x) \* (Array L' (S p))
+  end.
+
+Global Opaque Array.
+
+
+(* ---------------------------------------------------------------------- *)
+(** Array allocation *)
+
+Lemma Array_of_Alloc : forall k l,
+  Alloc k l ==>
+  \exists (L : list val), \[length L = k] \* Array L l.
+Proof using.
+  intros. gen l. induction k; intros.
+  { rew_Alloc. xsimpl (@nil val). rew_list~. }
+  { rew_Alloc. xpull ;=> v. xchange IHk. xpull ;=> L E.
+    xsimpl (v::L).
+    { rewrite Array_cons_eq. xsimpl~. }
+    { rew_list. math. } }
+Qed.
+
+Lemma triple_alloc_array : forall n,
+  n >= 0 ->
+  triple (val_alloc n)
+    \[]
+    (fun r => \exists (p:loc) (L:list val), \[r = val_loc p] \*
+              \[length L = n :> int] \* Array L p).
+Proof using.
+  introv N. xapp. math.
+  intros r. xpull ;=> l (E&Nl). subst r.
+  xchange Array_of_Alloc. xpull ;=> L HL.
+  xsimpl~. rewrite HL. rewrite~ abs_nonneg.
+Qed.
+
+
+
+
+(* ########################################################### *)
+(* ########################################################### *)
+(* ########################################################### *)
+(** * Additional contents *)
+
+
+(* ####################################################### *)
+(** ** Proof of operation on list cells *)
+
+(** *)
+
+Fixpoint MList (L:list val) (p:loc) : hprop :=
+  match L with
+  | nil => \[p = null]
+  | x::L' => \exists q, (p`.head ~~> x) \* (p`.tail ~~> q)
+                     \* (MList L' q)
+  end.
+
+Lemma MList_nil : forall p,
+  (p ~> MList nil) = \[p = null].
+Proof using. auto. Qed.
+
+Lemma MList_cons : forall p x L',
+  p ~> MList (x::L') =
+  \exists q, (p`.head ~~> x) \* (p`.tail ~~> q) \* MList L' q.
+Proof using.  auto. Qed.
+
+
+(** Next, we consider functions for constructing mutable lists.
+    We begin with the function that allocates one cell.
+    The function [mcell] takes as arguments the values to be
+    stored in the head and the tail fields of the new cell.
+
+[[
+    let rec mcell x q =
+      { head = x; tail = q }
+]]
+
+    In our ad-hoc program syntax, the [New] construct denotes record
+    allocation. *)
+
+Definition mcell : val :=
+  VFun 'x 'q :=
+    New`{ head := 'x ; tail := 'q }.
+
+(** The precondition of [mcell x q] is empty. Its postcondition
+    asserts that the return value is a location [p] such that
+    two fields are allocated: [p`.head ~~> x] and [p`.tail ~~> q]. *)
+
+Lemma Triple_mcell : forall (x:int) (q:loc),
+  TRIPLE (mcell x q)
+    PRE \[]
+    POST (fun (p:loc) => (p`.head ~~> x) \* (p`.tail ~~> q)).
+Proof using.
+  (* The tactic [xapp] handles the reasoning on the [New] construct. *)
+  xwp. xapp. xsimpl.
+Qed.
+
+Hint Extern 1 (Register_Spec mcell) => Provide Triple_mcell.
+
+(** The function [mcons] is an alias for [mcell].
+
+    Whereas [mcell] is intended to allocate a fresh cell on its own,
+    [mcons] is intended to extend an existing list by appending to
+    it a freshly-allocated cell. *)
+
+Definition mcons : val := mcell.
+
+(** The specification of [mcons] thus requires a list [q ~> MList L]
+    in its precondition, and produces a list [p ~> MList (x::L)] in
+    its postcondition. *)
+
+Lemma Triple_mcons : forall (x:int) (q:loc) (L:list int),
+  TRIPLE (mcons x q)
+    PRE (q ~> MList L)
+    POST (fun (p:loc) => p ~> MList (x::L)).
+Proof using.
+  intros. unfold mcons. xtriple. xapp Triple_mcell.
+  intros p. xchange <- MList_cons. (* Fold back the list *)
+Qed.
+
+Hint Extern 1 (Register_Spec mcons) => Provide Triple_mcons.
+
+
+
+
+(** The operation [mnil()] returns the [null] value.
+    The intention is to produce a representation for the empty list.
+
+[[
+    let rec mnil () =
+      null
+]]
+*)
+
+Definition mnil : val :=
+  VFun 'u :=
+    null.
+
+(** The precondition of [mnil] is empty. Its postcondition of [mnil]
+    asserts that the return value [p] is a pointer such that
+    [p ~> MList nil]. *)
+
+Lemma Triple_mnil :
+  TRIPLE (mnil '())
+    PRE \[]
+    POST (fun (p:loc) => p ~> MList nil).
+Proof using.
+  (* The proof requires introducing [null ~> MList nil] from nothing. *)
+  xwp. xval. xchange <- (MList_nil null). { auto. }
+Qed.
+
+Hint Extern 1 (Register_Spec mnil) => Provide Triple_mnil.
+
+(** Observe that the specification [Triple_mnil] does not mention
+    the [null] pointer anywhere. This specification can thus be
+    used to specify the behavior of operations on mutable lists
+    without having to reveal low-level implementation details. *)
+
+(** Remark: in the proof of [Triple_mnil], the call to
+    [xchange <- (MList_nil null)] can be replaced to a simpler
+    tactic invokation: [xchange MList_nil_intro], where
+    [MList_nil_intro] corresponds to the lemma stated next. *)
+
+Lemma MList_nil_intro :
+  \[] ==> (null ~> MList nil).
+Proof using. intros. xchange <- (MList_nil null). auto. Qed.
+
+Lemma Triple_mnil' :
+  TRIPLE (mnil '())
+    PRE \[]
+    POST (fun (p:loc) => p ~> MList nil).
+Proof using.
+  xwp. xval. xchange MList_nil_intro.
+Qed.
+
+
+
+(* ########################################################### *)
+(** ** List copy *)
+
+(** Let's put to practice the function [mnil] and [mcons] for
+    verifying the function [mcopy], which constructs an independent
+    copy of a given linked list.
+
+[[
+    let rec mcopy p =
+      if p == null
+        then mnil ()
+        else mcons (p.head) (mcopy p.tail)
+]]
+*)
+
+Definition mcopy : val :=
+  VFix 'f 'p :=
+    If_ 'p  '= null
+      Then mnil '()
+      Else mcons ('p'.head) ('f ('p'.tail)).
+
+(** The precondition of [mcopy] requires a linked list [p ~> MList L].
+    Its postcondition asserts that the function returns a pointer [p']
+    and a list [p' ~> MList L], in addition to the original list
+    [p ~> MList L]. The two lists are totally disjoint and independent,
+    as captured by the separating conjunction symbol (the star). *)
+
+Lemma Triple_mcopy : forall (p:loc) (L:list int),
+  TRIPLE (mcopy p)
+    PRE (p ~> MList L)
+    POST (fun (p':loc) => (p ~> MList L) \* (p' ~> MList L)).
+
+(** The proof script is very similar in structure to the previous ones.
+    While playing the script, try to spot the places where:
+
+    - [mnil] produces an empty list of the form [p' ~> MList nil],
+    - the recursive call produces a list of the form [q' ~> MList L'],
+    - [mcons] produces a list of the form [p' ~> MList (x::L')]. *)
+
+Proof using.
+  intros. gen p. induction_wf IH: list_sub L.
+  xwp. xapp. xchange MList_if. xif; intros C; case_if; xpull.
+  { intros ->. xapp. xsimpl. xchange* <- (MList_nil p). }
+  { intros x q L' ->. xapp. xapp. xapp*. intros q'.
+    xapp. intros p'. xchange <- MList_cons. }
+Qed.
+
+Hint Extern 1 (Register_Spec mcopy) => Provide Triple_mcopy.
+
+(* ########################################################### *)
+(** ** Deallocation of a cell: [mfree_cell] *)
+
+(** Separation Logic can be set up to enforce that all allocated data
+    eventually gets properly deallocated. In what follows, we describe
+    a function for deallocating one cell, and a function for deallocating
+    an entire mutable list. *)
+
+(** There is no explicit deallocation in OCaml, which is equipped with
+    a garbage collector, but let's pretend that there is a [delete]
+    operation for deallocating records.
+
+[[
+    let mfree_cell p =
+      delete p
+]]
+
+    For technical reasons (because our source language is untyped and our
+    formal semantics does not keep track of the size of allocated block),
+    we require in our ad-hoc program syntax the delete operation to
+    be annotated with the names of the fields of the record to be deleted,
+    as shown below.
+*)
+
+Definition mfree_cell : val :=
+  VFun 'p :=
+    val_dealloc 2 'p.
+
+Notation "'Delete' n" := (val_dealloc n) : trm_scope.
+
+(** The precondition of [mfree_cell p] describes the two fields
+    associated with the cell: [p`.head ~~> x] and [p`.tail ~~> q].
+    The postcondition is empty: the fields are destroyed. *)
+
+Lemma Triple_mfree_cell : forall (x:int) (p q:loc),
+  TRIPLE (mfree_cell p)
+    PRE ((p`.head ~~> x) \* (p`.tail ~~> q))
+    POST (fun (r:unit) => \[]).
+Proof using.
+  (* The tactic [xapp] handles the reasoning on the [Delete] construct. *)
+  xwp. xapp. xsimpl.
+Qed.
+
+Hint Extern 1 (Register_Spec mfree_cell) => Provide Triple_mfree_cell.
+
+
+(** The operation [mfree_list] deallocates all the cells in a given list.
+    It can be implemented as the following tail-recursive function.
+
+[[
+    let rec mfree_list p =
+      if p != null then begin
+        let q = p.tail in
+        mfree_cell p;
+        mfree_list q
+      end
+]]
+
+*)
+
+Definition mfree_list : val :=
+  VFix 'f 'p :=
+    If_ 'p '<> null Then
+      Let 'q := 'p'.tail in
+      mfree_cell 'p ';
+      'f 'q
+    End.
+
+(** The precondition of [mfree_list p] requires a full list [p ~> MList L].
+    The postcondition is empty: the entire list is destroyed. *)
+
+(* EX1! (Triple_mfree_list) *)
+(** Verify the function [mfree_list].
+    Hint: follow the pattern of the proof of the function [mlength]. *)
+
+Lemma Triple_mfree_list : forall (p:loc) (L: list int),
+  TRIPLE (mfree_list p)
+    PRE (p ~> MList L)
+    POST (fun (r:unit) => \[]).
+Proof using. (* ADMITTED *)
+  intros. gen p. induction_wf IH: list_sub L. intros.
+  xwp. xchange MList_if. xif; intros C; case_if; xpull.
+  { intros x p' L' ->. xapp. xapp. xapp. { auto. } xsimpl. }
+  { intros ->. xval. xsimpl. }
+Qed. (* /ADMITTED *)
+
+(** [] *)
+
+Hint Extern 1 (Register_Spec mfree_list) => Provide Triple_mfree_list.
+
+(** This concludes our quick tour of functions on mutable lists.
+    Additional functions are presented further in the file,
+    as exercises. *)
+
+
+(* ####################################################### *)
+(** ** Local reasoning on arrays *)
+
+Lemma Array_nil_eq : forall p,
+  Array nil p = \[].
+Proof using. auto. Qed.
+
+Lemma Array_cons_eq : forall p x L,
+  Array (x::L) p = (p ~~~> x) \* Array L (S p).
+Proof using. auto. Qed.
+
+Lemma Array_one_eq : forall p x,
+  Array (x::nil) p = (p ~~~> x).
+Proof using. intros. rewrite Array_cons_eq, Array_nil_eq. rew_heap~. Qed.
+
+Lemma Array_concat_eq : forall p L1 L2,
+  Array (L1++L2) p = Array L1 p \* Array L2 (p + length L1)%nat.
+Proof using.
+  Transparent loc.
+  intros. gen p. induction L1; intros; rew_list.
+  { rewrite Array_nil_eq. rew_heap. fequals. unfold loc; math. }
+  { do 2 rewrite Array_cons_eq. rewrite IHL1. rew_heap. do 3 fequals.
+    unfold loc; math. }
+Qed.
+
+Lemma Array_last_eq : forall p x L,
+  Array (L&x) p = Array L p \* ((p + length L)%nat ~~~> x).
+Proof using. intros. rewrite Array_concat_eq. rewrite~ Array_one_eq. Qed.
+
+Lemma Array_middle_eq : forall n p L,
+  0 <= n < length L ->
+  Array L p = \exists L1 x L2, \[L = L1++x::L2] \* \[length L1 = n :> int] \*
+    Array L1 p \* (abs(p+n) ~~~> x) \* Array L2 (p + length L1 + 1)%nat.
+Proof using.
+  (* LATER: simplify the Z/nat math, by using a result from LibListZ directly *)
+  introv N. applys himpl_antisym.
+  { forwards (L1&x&L2&E&HM): list_middle_inv (abs n) L.
+    asserts (N1&N2): (0 <= abs n /\ (abs n < length L)%Z).
+    { split; rewrite abs_nonneg; math. } math.
+    lets M': eq_int_of_eq_nat HM. rewrite abs_nonneg in M'; [|math].
+    xsimpl~ (>> L1 x L2). subst L. rewrite Array_concat_eq, Array_cons_eq.
+    rew_nat. xsimpl. rewrite HM. rewrite~ abs_nat_plus_nonneg. math. }
+  { xpull ;=> L1 x L2 HM E. subst n.
+    subst L. rewrite Array_concat_eq, Array_cons_eq.
+    rew_nat. xsimpl. applys_eq himpl_refl 1. fequals.
+    rewrite abs_nat_plus_nonneg; [|math]. rewrite~ abs_nat. }
+Qed.
+
+function count
+
+parallel calls remark
+
+
+(* ########################################################### *)
+(* ########################################################### *)
+(* ########################################################### *)
+(** * Bonus contents (optional reading) *)
+
+
+(* ########################################################### *)
+(** ** Semantics of the allocation operations *)
+
+
+  | eval_alloc : forall k n ma mb l,
+      mb = Fmap.conseq l (LibList.make k val_uninitialized) ->
+      n = nat_to_Z k ->
+      l <> null ->
+      Fmap.disjoint ma mb ->
+      eval ma (val_alloc (val_int n)) (mb \+ ma) (val_loc l)
+  | eval_dealloc : forall n vs ma mb l,
+      mb = Fmap.conseq l vs ->
+      n = LibList.length vs ->
+      Fmap.disjoint ma mb ->
+      eval (mb \+ ma) (val_dealloc (val_int n) (val_loc l)) ma val_unit.
+
+
+Lemma Alloc_fmap_conseq : forall l k,
+  l <> null ->
+  (Alloc k l) (Fmap.conseq l (LibList.make k val_uninitialized)).
+Proof using.
+  Transparent loc null.
+  introv N. gen l. induction k; intros; rew_Alloc.
+  { rewrite LibList.make_zero, Fmap.conseq_nil. applys~ hempty_intro. }
+  { rewrite LibList.make_succ, Fmap.conseq_cons. applys hstar_intro.
+    { split~. }
+    { applys IHk. unfolds loc, null. math. }
+    { applys~ Fmap.disjoint_single_conseq. } }
+Qed.
+
+
+
+
+(* ########################################################### *)
+(** ** Definition of record operations using pointer arithmetics *)
+
+Definition val_get_field (k:field) : val :=
+  VFun 'p :=
+    Let 'q := val_ptr_add 'p (nat_to_Z k) in
+    val_get 'q.
+
+Definition val_set_field (k:field) : val :=
+  VFun 'p 'v :=
+    Let 'q := val_ptr_add 'p (nat_to_Z k) in
+    val_set 'q 'v.
+
+End FieldAccessDef.
+
+Notation "t1 ''.' f" :=
+  (val_get_field f t1)
+  (at level 56, f at level 0, format "t1 ''.' f" ) : trm_scope.
+
+Notation "'Set' t1 ''.' f '':=' t2" :=
+  (val_set_field f t1 t2)
+  (at level 65, t1 at level 0, f at level 0, format "'Set' t1 ''.' f  '':=' t2") : trm_scope.
+
+Lemma triple_get_field : forall l f v,
+  triple ((val_get_field f) l)
+    (l`.f ~~> v)
+    (fun r => \[r = v] \* (l`.f ~~> v)).
+Proof using.
+  xwp. xapp. unfold hfield. xpull. intros N. xapp. xsimpl*.
+Qed.
+
+Lemma triple_set_field : forall v1 l f v2,
+  triple ((val_set_field f) l v2)
+    (l`.f ~~> v1)
+    (fun _ => l`.f ~~> v2).
+Proof using.
+  xwp. xapp. unfold hfield. xpull. intros N. xapp. xsimpl*.
+Qed.
+
+
+(* ########################################################### *)
+(** ** Definition of array operations using pointer arithmetics *)
+
+
+(* -------------------------------------------------------------------------- *)
+(** Accesses *)
+
+Import LibListZ.
+Implicit Types i ofs len : int.
+
+
+(* ---------------------------------------------------------------------- *)
+(** Array get *)
+
+Definition val_array_get : val :=
+  ValFun 'p 'i :=
+    Let 'n := val_ptr_add 'p 'i in
+    val_get 'n.
+
+Lemma triple_array_get : forall p i L,
+  index L i ->
+  triple (val_array_get p i)
+    (Array L p)
+    (fun r => \[r = L[i]] \* Array L p).
+Proof using.
+  introv N. rewrite index_eq_inbound in N.
+  xcf. xapps. { math. }
+  rewrites (>> Array_middle_eq i). { math. }
+  xtpull ;=> L1 x L2 EL HL.
+  xapp. xpull ;=> r. intro_subst.
+  xsimpl; auto. { subst. rewrite~ read_middle. }
+Qed.
+
+Hint Extern 1 (Register_spec val_array_get) => Provide triple_array_get.
+
+Notation "'Array'' p `[ i ]" := (trm_app (trm_app (trm_val val_array_get) p) i)
+  (at level 69, p at level 0, no associativity,
+   format "'Array''  p `[ i ]") : charac.
+
+
+(* ---------------------------------------------------------------------- *)
+(** Array set *)
+
+Definition val_array_set : val :=
+  ValFun 'p 'i 'x :=
+    Let 'n := val_ptr_add 'p 'i in
+    val_set 'n 'x.
+
+Lemma triple_array_set : forall p i v L,
+  index L i ->
+  triple (val_array_set p i v)
+    (Array L p)
+    (fun r => \[r = val_unit] \* Array (L[i:=v]) p).
+Proof using.
+  introv N. rewrite index_eq_inbound in N.
+  xcf. xapps. { math. }
+  rewrites (>> Array_middle_eq i). { math. }
+  xtpull ;=> L1 x L2 EL HL.
+  xapp triple_set. xpull ;=> r. intro_subst.
+  rewrites (>> Array_middle_eq i (L[i := v])).
+   { rewrite <- length_eq in *. rew_array. math. }
+  xsimpl; auto. { subst. rewrite~ update_middle. rew_list~. }
+Qed.
+
+Hint Extern 1 (Register_spec val_array_set) => Provide triple_array_set.
+
+Notation "'Array'' p `[ i ] `<- x" := (trm_app (trm_app (trm_app (trm_val val_array_set) p) i) x)
+  (at level 69, p at level 0, no associativity,
+   format "'Array''  p `[ i ]  `<-  x") : charac.
+
+
+(* ---------------------------------------------------------------------- *)
+(** Array make *)
+
+Definition val_array_make : val :=
+  ValFun 'n 'v :=
+    Let 'p := val_alloc 'n in
+    Let 'b := 'n '- 1 in
+    For 'i := 0 To 'b Do
+      Array' 'p`['i] `<- 'v
+    Done;;;
+    'p.
+
+(* ####################################################### *)
+(** ** Grouped representation of record fields *)
+
+
+(** Representation predicate [r ~> Record L], where [L]
+    is an association list from fields to values. *)
+
+Definition Record_field : Type := field * dyn.
+Definition Record_fields : Type := list Record_field.
+
+Bind Scope fields_scope with Record_fields.
+
+Fixpoint Record (L:Record_fields) (r:loc) : hprop :=
+  match L with
+  | nil => \[]
+  | (f, Dyn V)::L' => (r`.f ~~> V) \* (r ~> Record L')
+  end.
+
+(* --TODO: currently restricted due to [r `. f ~> V] not ensuring [r<>null] *)
+(* --TODO: rename *)
+Lemma hRecord_not_null : forall (r:loc) (L:Record_fields),
+  (* L <> nil -> *)
+  mem (0%nat:field) (List.map fst L) ->
+  (r ~> Record L) ==> (r ~> Record L) \* \[r <> null].
+Proof using.
+  introv M. induction L as [|(f,[A EA v]) L'].
+  { inverts M. }
+  { xunfold Record. inverts M.
+    { xchange~ (Hfield_not_null r). xsimpl~. }
+    { xchange~ IHL'. xsimpl~. } }
+Qed.
+
+(** Lemmas for unfolding the definition *)
+
+Lemma Record_nil : forall p,
+  p ~> Record nil = \[].
+Proof using. auto. Qed.
+
+Lemma Record_cons : forall p x (V:dyn) L,
+  (p ~> Record ((x, V)::L)) =
+  (p`.x ~~> ``V \* p ~> Record L).
+Proof using. intros. destruct~ V. Qed.
+
+Hint Rewrite Record_nil Record_cons enc_dyn_make : Record_to_HField.
+
+
+Local Open Scope heap_scope_ext.
+
+Lemma Record_not_null : forall (r:loc) (L:Record_fields),
+  L <> nil ->
+  (r ~> Record L) ==+> \[r <> null].
+Proof using.
+  intros. destruct L as [|(f,v) L']. { false. }
+  rewrite Record_cons. xchanges~ Hfield_not_null.
+Qed.
+
+
+
+(* ####################################################### *)
+(** ** Treatment of uncurried functions *)
+
+  | trm_fixs : var -> list var -> trm -> trm
+  | trm_apps : trm -> list trm -> trm
+
+
+Fixpoint subst (y:var) (w:val) (t:trm) : trm :=
+  let aux t :=
+    subst y w t in
+  let aux_no_captures xs t :=
+    If LibList.mem y xs then t else aux t in
+  match t with
+  | trm_fixs f xs t1 => trm_fixs f xs (If f = y then t1 else
+                                        aux_no_captures xs t1)
+  | trm_apps t0 ts => trm_apps (aux t0) (List.map aux ts)
+  ...
+ end.
+
+
+Lemma subst_trm_fixs : forall y w f xs t,
+  var_fresh y (f::xs) ->
+  subst1 y w (trm_fixs f xs t) = trm_fixs f xs (subst1 y w t).
+Proof using.
+  introv N. simpls. case_var.
+  { false* var_fresh_mem_inv. }
+  { auto. }
+Qed.
+
+
+  | eval_fixs : forall m f xs t1,
+      xs <> nil ->
+      eval m (trm_fixs f xs t1) m (val_fixs f xs t1)
+
+  | eval_apps_fixs : forall m1 m2 f xs t3 v0 vs r,
+      v0 = val_fixs f xs t3 ->
+      var_fixs f (length vs) xs ->
+      eval m1 (substn xs vs (subst1 f v0 t3)) m2 r ->
+      eval m1 (trm_apps v0 vs) m2 r
+
+
+Fixpoint var_distinct (xs:vars) : Prop :=
+  match xs with
+  | nil => True
+  | x::xs' => var_fresh x xs' /\ var_distinct xs'
+  end.
+
+Fixpoint var_fresh (y:var) (xs:vars) : bool :=
+  match xs with
+  | nil => true
+  | x::xs' => if var_eq x y then false else var_fresh y xs'
+  end.
+
+
+(** [noduplicates L] asserts that [L] does not contain any
+    duplicated item. *)
+
+Inductive noduplicates A : list A -> Prop :=
+  | noduplicates_nil : noduplicates nil
+  | noduplicates_cons : forall x l,
+      ~ (mem x l) ->
+      noduplicates l ->
+      noduplicates (x::l).
+
+
+
+Definition var_fixs (f:var) (n:nat) (xs:vars) : Prop :=
+     var_distinct (f::xs)
+  /\ length xs = n
+  /\ xs <> nil.
+
+Definition var_fixs_exec (f:bind) (n:nat) (xs:vars) : bool := ..
+
+Lemma var_fixs_exec_eq : forall f (n:nat) xs,
+  var_fixs_exec f n xs = isTrue (var_fixs f n xs).
+
+
+Lemma triple_apps_fixs : forall xs (f:var) F (Vs:vals) t1 H Q,
+  F = (val_fixs f xs t1) ->
+  var_fixs f (length Vs) xs ->
+  triple (substn (f::xs) (F::Vs) t1) H Q ->
+  triple (trm_apps F Vs) H Q.
+Proof using.
+  introv E N M. intros H' h Hf. forwards (h'&v&R&K): (rm M) Hf.
+  exists h' v. splits~. { subst. applys* eval_apps_fixs. }
+Qed.
+
+
+Fixpoint trms_to_vals_rec (acc:vals) (ts:trms) : option vals :=
+  match ts with
+  | nil => Some (List.rev acc)
+  | trm_val v :: ts' => trms_to_vals_rec (v::acc) ts'
+  | _ => None
+  end.
+
+Definition trms_to_vals (ts:trms) : option vals :=
+  trms_to_vals_rec nil ts.
+
+
+Lemma xwp_lemma_fixs : forall F f vs ts xs t H Q,
+  F = val_fixs f xs t ->
+  trms_to_vals ts = Some vs ->
+  var_fixs_exec f (length vs) xs ->
+  H ==> (wpgen (combine (f::xs) (F::vs)) t) Q ->
+  triple (trm_apps F ts) H Q.
+
+
+(* ####################################################### *)
+(** ** Coercion for uncurried functions *)
+
+Coercion trm_to_pat : trm >-> pat.
+
+(** Parsing facility: coercions for turning [t1 t2 t3]
+    into [trm_apps t1 (t2::t3::nil)] *)
+
+Inductive combiner :=
+  | combiner_nil : trm -> trm -> combiner
+  | combiner_cons : combiner -> trm -> combiner.
+
+Coercion combiner_nil : trm >-> Funclass.
+Coercion combiner_cons : combiner >-> Funclass.
+
+Fixpoint combiner_to_trm (c:combiner) : trm :=
+  match c with
+  | combiner_nil t1 t2 => trm_apps t1 (t2::nil)
+  | combiner_cons c1 t2 =>
+      match combiner_to_trm c1 with
+      | trm_apps t1 ts => trm_apps t1 (List.app ts (t2::nil))
+      | t1 => trm_apps t1 (t2::nil)
+      end
+  end.
+
+Coercion combiner_to_trm : combiner >-> trm.
+
+
+
+*)
